core-lan-sem-coind-conv.v
@@ -1,0 +1,1694 @@
+From Coq Require Import List Arith Lia.
+Import ListNotations.
+From Paco Require Import paco.
+
+(* ================================================== *)
+(* 1) Syntax: smaller language (dependent + NatRec)   *)
+(* ================================================== *)
+
+Inductive term : Type :=
+  | Star : term
+  | Nat  : term
+  | Pi : term -> term -> term
+  | Zero : term
+  | Succ : term -> term
+  | Var : nat -> term
+  | Lam : term -> term -> term
+  | App : term -> term -> term
+  | NatRec : term -> term -> term -> term -> term  (* P z s n *)
+  | Vec : term -> term -> term                (* Vec A n  *)
+  | Nil : term -> term                        (* Nil A     *)
+  | Cons : term -> term -> term -> term -> term     (* Cons A n x xs *)
+  | VecRec : term -> term -> term -> term -> term -> term.
+
+Inductive whnf : Type :=
+| VStar  : whnf
+| VNat   : whnf
+| VPi    : whnf -> closure -> whnf
+| VLam   : whnf -> closure -> whnf
+| VZero  : whnf
+| VSucc  : whnf -> whnf
+| VNeutral : neutral -> whnf
+| VVec  : whnf -> whnf -> whnf              (* VVec vA vn *)
+| VNil  : whnf -> whnf                      (* VNil vA *)
+| VCons : whnf -> whnf -> whnf -> whnf -> whnf    (* VCons vA vn vx vxs *)
+
+with neutral : Type :=
+| NVar : nat -> neutral
+| NApp : neutral -> whnf -> neutral
+| NNatRec : whnf -> whnf -> whnf -> neutral -> neutral
+| NVecRec : whnf -> whnf -> whnf -> whnf -> neutral -> neutral
+
+with closure : Type :=
+| Cl : list whnf -> term -> closure.
+
+Coercion VNeutral : neutral >-> whnf.
+
+Section ManualMutualInduction_Prop.
+
+  Variable Pw : whnf -> Prop.
+  Variable Pn : neutral -> Prop.
+  Variable Pc : closure -> Prop.
+
+  (* Hypotheses for each constructor (one hypothesis per constructor) *)
+  Hypotheses
+    (H_VStar    : Pw VStar)
+    (H_VNat     : Pw VNat)
+    (H_VPi      : forall A B, Pw A -> Pc B -> Pw (VPi A B))
+    (H_VLam     : forall A cl, Pw A ->  Pc cl -> Pw (VLam A cl))
+    (H_VZero    : Pw VZero)
+    (H_VSucc    : forall n, Pw n -> Pw (VSucc n))
+    (H_VNeutral : forall n, Pn n -> Pw (VNeutral n))
+
+    (* --- vector WHNFs --- *)
+    (H_VVec  : forall vA vn, Pw vA -> Pw vn -> Pw (VVec vA vn))
+    (H_VNil  : forall vA, Pw vA -> Pw (VNil vA))
+    (H_VCons : forall vA vn vx vxs,Pw vA -> Pw vn -> Pw vx -> Pw vxs -> Pw (VCons vA vn vx vxs))
+
+    (H_NVar    : forall i, Pn (NVar i))
+    (H_NApp    : forall n v, Pn n -> Pw v -> Pn (NApp n v))
+    (H_NNatRec : forall P z s n, Pw P -> Pw z -> Pw s -> Pn n -> Pn (NNatRec P z s n))
+    (H_NVecRec : forall vP vnil vcons vinx nn, Pw vP -> Pw vnil -> Pw vcons -> Pw vinx -> Pn nn -> Pn (NVecRec vP vnil vcons vinx nn))
+
+    (H_Cl     : forall ρ t, Forall Pw ρ -> Pc (Cl ρ t)).
+
+  (* Helper: build a Forall Pw ρ by structural recursion over the list ρ,
+     using the mutual whnf_proof function for elements. *)
+
+  Fixpoint whnf_proof (v : whnf) {struct v} : Pw v :=
+    match v with
+    | VStar            => H_VStar
+    | VNat             => H_VNat
+    | VPi A B          => H_VPi A B (whnf_proof A) (closure_proof B)
+    | VLam A cl        => H_VLam A cl (whnf_proof A) (closure_proof cl)
+    | VZero            => H_VZero
+    | VSucc n          => H_VSucc n (whnf_proof n)
+    | VNeutral n       => H_VNeutral n (neutral_proof n)
+    | VVec vA vn       => H_VVec vA vn (whnf_proof vA) (whnf_proof vn)
+    | VNil vA          => H_VNil vA (whnf_proof vA)
+    | VCons vA vn vx vxs => H_VCons vA vn vx vxs (whnf_proof vA) (whnf_proof vn) (whnf_proof vx) (whnf_proof vxs)
+    end
+
+  with neutral_proof (n : neutral) {struct n} : Pn n :=
+    match n with
+    | NVar i           => H_NVar i
+    | NApp n' v        => H_NApp n' v (neutral_proof n') (whnf_proof v)
+    | NNatRec P z s n' => H_NNatRec P z s n' (whnf_proof P) (whnf_proof z) (whnf_proof s) (neutral_proof n')
+    | NVecRec P z s vinx n' => H_NVecRec P z s vinx n' (whnf_proof P) (whnf_proof z) (whnf_proof s) (whnf_proof vinx) (neutral_proof n')
+
+    end
+
+  with closure_proof (c : closure) {struct c} : Pc c :=
+    match c with
+    | Cl ρ t =>
+        (* local structural recursion over ρ that may call whnf_proof for each head *)
+        let fix build (ρ0 : list whnf) : Forall Pw ρ0 :=
+            match ρ0 with
+            | []     => @Forall_nil whnf Pw
+            | v :: r => @Forall_cons whnf Pw v r (whnf_proof v) (build r)
+            end
+        in H_Cl ρ t (build ρ)
+    end.
+
+  Theorem whnf_mutind :
+    (forall v, Pw v) /\ (forall n, Pn n) /\ (forall c, Pc c).
+  Proof.
+    split.
+    - intro v; exact (whnf_proof v).
+    - split.
+      + intro n; exact (neutral_proof n).
+      + intro c; exact (closure_proof c).
+  Qed.
+
+End ManualMutualInduction_Prop.
+
+
+(* ----------------------------------------------------------------- *)
+(*  Runtime application and evaluation (no dependency on vconv/closure_conv) *)
+(* ----------------------------------------------------------------- *)
+
+(* vapp: only two runtime shapes: real lambda closures, or neutral app *)
+Inductive vapp : whnf -> whnf -> whnf -> Prop :=
+| VApp_Lam_sharp : forall vA clρ body ρ arg vres,
+    (* apply a real lambda closure: evaluate body in arg :: env_of_cl cl *)
+    clρ = Cl ρ body ->
+    eval' (arg :: ρ) body vres ->
+    vapp (VLam vA clρ) arg vres
+| VApp_Pi_sharp : forall vA ρ body arg vres,
+    eval' (arg :: ρ) body vres ->
+    vapp (VPi vA (Cl ρ body)) arg vres
+
+| VApp_Neut_sharp : forall n v,
+    vapp (VNeutral n) v (VNeutral (NApp n v))
+
+(* evaluation for natrec (observational, using vapp which only inspects VLam/VNeutral) *)
+with eval_natrec : whnf -> whnf -> whnf -> whnf -> whnf -> Prop :=
+| ENR_Zero : forall vP vz vs,
+    eval_natrec vP vz vs VZero vz
+| ENR_Succ : forall vP vz vs vn vrec v1 v,
+    eval_natrec vP vz vs vn vrec ->
+    vapp vs vn v1 ->
+    vapp v1 vrec v ->
+    eval_natrec vP vz vs (VSucc vn) v
+| ENR_Neut : forall vP vz vs nn,
+    eval_natrec vP vz vs (VNeutral nn) (VNeutral (NNatRec vP vz vs nn))
+
+(* evaluation for vecrec (observational, using vapp) *)
+with eval_vecrec : whnf -> whnf -> whnf -> whnf -> whnf -> whnf -> Prop :=
+| EVR_Nil : forall vP vnil vcons vindex vA,
+    eval_vecrec vP vnil vcons vindex (VNil vA) vnil
+
+| EVR_Cons : forall vP vnil vcons vindex vA vn vx vxs vrec v1 v2 v,
+    eval_vecrec vP vnil vcons vindex vxs vrec ->
+    vapp vcons vx v1 ->
+    vapp v1 vxs v2 ->
+    vapp v2 vrec v ->
+    eval_vecrec vP vnil vcons vindex (VCons vA vn vx vxs) v
+
+| EVR_Neut : forall vP vnil vcons vindex nn,
+    eval_vecrec vP vnil vcons vindex (VNeutral nn) (VNeutral (NVecRec vP vnil vcons vindex nn))
+
+(* ----------------------------------------------------------------- *)
+(*  eval' : big-step evaluator to WHNF (no use of closure_conv/vconv) *)
+(* ----------------------------------------------------------------- *)
+with eval' : list whnf -> term -> whnf -> Prop :=
+| E'_Star : forall ρ, eval' ρ Star VStar
+| E'_Nat : forall ρ, eval' ρ Nat VNat
+
+| E'_Var_Some : forall ρ x v,
+    nth_error ρ x = Some v ->
+    eval' ρ (Var x) v
+
+| E'_Var_None : forall ρ x,
+    nth_error ρ x = None ->
+    eval' ρ (Var x) (VNeutral (NVar (x - length ρ)))
+
+| E'_Pi : forall ρ A B vA,
+    eval' ρ A vA ->
+    eval' ρ (Pi A B) (VPi vA (Cl ρ B))
+
+| E'_Lam : forall ρ A vA b,
+    eval' ρ A vA ->
+    eval' ρ (Lam A b) (VLam vA (Cl ρ b))
+
+| E'_App : forall ρ t u vt vu v,
+    eval' ρ t vt ->
+    eval' ρ u vu ->
+    vapp vt vu v ->
+    eval' ρ (App t u) v
+
+| E'_Zero : forall ρ, eval' ρ Zero VZero
+
+| E'_Succ : forall ρ n vn,
+    eval' ρ n vn ->
+    eval' ρ (Succ n) (VSucc vn)
+
+| E'_NatRec : forall ρ P z s n vP vz vs vn v,
+    eval' ρ P vP ->
+    eval' ρ z vz ->
+    eval' ρ s vs ->
+    eval' ρ n vn ->
+    eval_natrec vP vz vs vn v ->
+    eval' ρ (NatRec P z s n) v
+
+| E'_Vec : forall ρ A n vA vn,
+    eval' ρ A vA ->
+    eval' ρ n vn ->
+    eval' ρ (Vec A n) (VVec vA vn)
+
+| E'_Nil : forall ρ A vA,
+    eval' ρ A vA ->
+    eval' ρ (Nil A) (VNil vA)
+
+| E'_Cons : forall ρ A n x xs vA vn vx vxs,
+    eval' ρ A vA ->
+    eval' ρ n vn ->
+    eval' ρ x vx ->
+    eval' ρ xs vxs ->
+    eval' ρ (Cons A n x xs) (VCons vA vn vx vxs)
+
+| E'_VecRec : forall ρ P nil cons n t vt vP vnil vcons vn vres,
+    eval' ρ P vP ->
+    eval' ρ nil vnil ->
+    eval' ρ cons vcons ->
+    eval' ρ n vn ->
+    eval' ρ t vt ->
+    eval_vecrec vP vnil vcons vn vt vres ->
+    eval' ρ (VecRec P nil cons n t) vres.
+
+Scheme eval'_rect := Induction for eval' Sort Prop
+with vapp_rect := Induction for vapp Sort Prop
+with eval_natrec_rect := Induction for eval_natrec Sort Prop
+with eval_vecrec_rect := Induction for eval_vecrec Sort Prop.
+
+Combined Scheme evals_mutind from eval'_rect, vapp_rect, eval_natrec_rect, eval_vecrec_rect.
+
+
+Lemma evals_deterministic :
+  (forall ρ t v1, eval' ρ t v1 -> forall v2, eval' ρ t v2 -> v1 = v2)
+  /\
+  (forall vt arg r1, vapp vt arg r1 -> forall r2, vapp vt arg r2 -> r1 = r2)
+  /\
+  (forall vP vz vs n r1, eval_natrec vP vz vs n r1 -> forall r2, eval_natrec vP vz vs n r2 -> r1 = r2)
+  /\
+  (forall vP vnil vcons vindex t r1,
+     eval_vecrec vP vnil vcons vindex t r1 ->
+     forall r2, eval_vecrec vP vnil vcons vindex t r2 -> r1 = r2).
+Proof.
+  apply evals_mutind; intros.
+(*   apply (evals_mutind
+    (fun ρ t v _ => forall v', eval' ρ t v' -> v = v')
+    (fun vt arg r _ => forall r', vapp vt arg r' -> r = r')
+    (fun vP vz vs n v _ => forall v', eval_natrec vP vz vs n v' -> v = v')
+    (fun vP vnil vcons vindex vt v _ =>
+       forall v', eval_vecrec vP vnil vcons vindex vt v' -> v = v')). *)
+   23:{
+   intros.
+   inversion H. subst. easy.
+   }
+   22:{
+   intros.
+   inversion H3. subst.
+   apply H in H12.
+   apply H0 in H14.
+   subst.
+   apply H1 in H15.
+   subst.
+   apply H2 in H16.
+   easy.
+   }
+   21:{
+   inversion H. subst. easy.
+   }
+   20:{
+   inversion H. subst. easy.
+   }
+   19:{
+   inversion H2. subst.
+   apply H in H4.
+   apply H0 in H5. subst.
+   apply H1 in H9.
+   easy.
+   }
+   18:{
+   inversion H. easy.
+   }
+   17:{
+   inversion H. easy.
+   }
+   16:{
+   inversion H0. subst.
+   apply H. (* inversion H3. *) easy.
+   }
+   15:{
+   inversion H0. subst.
+   apply H. inversion H3. easy.
+   }
+   14:{
+   inversion H5. subst.
+   apply H in H11.
+   apply H0 in H13.
+   apply H1 in H15.
+   apply H2 in H16.
+   apply H3 in H17. subst.
+   apply H4 in H18. easy.
+   }
+   13:{
+   inversion H3. subst.
+   apply H in H9.
+   apply H0 in H11.
+   apply H1 in H12.
+   apply H2 in H13.
+   subst. easy.
+   }
+   12:{
+   inversion H0. subst.
+   apply H in H3.
+   subst. easy.
+   }
+   11:{
+   inversion H1. subst.
+   apply H in H5.
+   apply H0 in H7. subst.
+   easy.
+   }
+   10:{
+   inversion H4. subst.
+   apply H in H9.
+   apply H0 in H11.
+   apply H1 in H13.
+   apply H2 in H14.
+   subst.
+   apply H3 in H15. easy.
+   }
+   9:{
+   inversion H0. subst.
+   apply H in H3. subst. easy.
+   }
+   8:{
+   inversion H. easy.
+   }
+   7:{
+   inversion H2. subst.
+   apply H in H5.
+   apply H0 in H7. subst.
+   apply H1 in H9.
+   easy.
+   }
+   6:{
+   inversion H0. subst.
+   apply H in H5. subst. easy.
+   }
+   5:{
+   inversion H0. subst.
+   apply H in H5. subst.
+   easy.
+   }
+   4:{
+   inversion H.
+   + subst. rewrite e in H2. easy.
+   + subst. easy.
+   }
+   3:{
+   inversion H. 
+   + subst. rewrite e in H2. inversion H2. easy.
+   + subst. rewrite e in H2. easy.
+   }
+   2:{
+   inversion H. easy.
+   }
+   1:{
+   inversion H. easy.
+   }
+Qed.
+
+Definition eval'_det :
+  forall ρ t v1 v2,
+    eval' ρ t v1 -> eval' ρ t v2 -> v1 = v2.
+Proof. destruct evals_deterministic as [H _]. eauto. Qed.
+
+Definition vapp_det :
+  forall vt arg r1 r2,
+    vapp vt arg r1 -> vapp vt arg r2 -> r1 = r2.
+Proof.
+  destruct evals_deterministic as [_ [H _]].
+  eauto.
+Qed.
+
+Definition eval_natrec_det :
+  forall vP vz vs n r1 r2,
+    eval_natrec vP vz vs n r1 -> eval_natrec vP vz vs n r2 -> r1 = r2.
+Proof.
+  destruct evals_deterministic as [_ [_ [H _]]].
+  eauto.
+Qed.
+
+Definition eval_vecrec_det :
+  forall vP vnil vcons vindex t r1 r2,
+    eval_vecrec vP vnil vcons vindex t r1 ->
+    eval_vecrec vP vnil vcons vindex t r2 ->
+    r1 = r2.
+Proof.
+  destruct evals_deterministic as [_ [_ [_ H]]].
+  eauto.
+Qed.
+
+(* ------------------------------------------------------------------ *)
+(* Tag all three relation kinds into one type so we can use paco2 on  *)
+(* a single binary relation over these tags; projections give the real *)
+(* three relations.                                                     *)
+(* ------------------------------------------------------------------ *)
+
+Inductive conv_tag : Type :=
+| TNe : neutral -> conv_tag
+| TV  : whnf -> conv_tag
+| TC  : closure -> conv_tag.
+
+(* accessors (you already have equivalents; we include here for completeness) *)
+Definition env_of_cl (cl : closure) : list whnf :=
+  match cl with Cl rho _ => rho end.
+
+Definition body_of_cl (cl : closure) : term :=
+  match cl with Cl _ t => t end.
+
+(* ------------------------------------------------------------------ *)
+(* The functor F: (conv_tag -> conv_tag -> Prop) -> conv_tag -> conv_tag -> Prop
+   It describes one unfolding step of the mutually coinductive relations.
+   We write it so recursive occurrences refer to "r x y".               *)
+(* ------------------------------------------------------------------ *)
+
+Definition convF
+  (r : conv_tag -> conv_tag -> Prop)
+  (x y : conv_tag) : Prop :=
+
+  match x, y with
+
+  (* neutral cases *)
+  | TNe (NVar i), TNe (NVar j) =>
+      (* only equal when same var index *)
+      i = j
+
+  | TNe (NApp n1 v1), TNe (NApp n2 v2) =>
+      (* n1 ~ n2 as neutrals, and v1 ~ v2 as values (use r on TV) *)
+      r (TNe n1) (TNe n2) /\ r (TV v1) (TV v2)
+
+  | TNe (NNatRec P1 z1 s1 n1), TNe (NNatRec P2 z2 s2 n2) =>
+      r (TV P1) (TV P2) /\ r (TV z1) (TV z2) /\ r (TV s1) (TV s2) /\ r (TNe n1) (TNe n2)
+
+  | TNe (NVecRec P1 nil1 cons1 idx1 n1), TNe (NVecRec P2 nil2 cons2 idx2 n2) =>
+      r (TV P1) (TV P2) /\ r (TV nil1) (TV nil2) /\ r (TV cons1) (TV cons2) /\ r (TV idx1) (TV idx2) /\ r (TNe n1) (TNe n2)
+
+  (* value cases *)
+  | TV VStar, TV VStar => True
+  | TV VNat,  TV VNat  => True
+  | TV VZero, TV VZero => True
+
+  | TV (VSucc n1), TV (VSucc n2) =>
+      r (TV n1) (TV n2)
+
+  | TV (VNeutral n1), TV (VNeutral n2) =>
+      r (TNe n1) (TNe n2)
+
+  | TV (VVec a1 n1), TV (VVec a2 n2) =>
+      r (TV a1) (TV a2) /\ r (TV n1) (TV n2)
+
+  | TV (VNil a1), TV (VNil a2) =>
+      r (TV a1) (TV a2)
+
+  | TV (VCons a1 n1 x1 xs1), TV (VCons a2 n2 x2 xs2) =>
+      r (TV a1) (TV a2) /\ r (TV n1) (TV n2) /\ r (TV x1) (TV x2) /\ r (TV xs1) (TV xs2)
+
+  (* Lam-Lam and Pi-Pi via closure_conv (use r on TC) *)
+  | TV (VLam vA1 cl1), TV (VLam vA2 cl2) =>
+      r (TV vA1) (TV vA2) /\ r (TC cl1) (TC cl2)
+
+  | TV (VPi vA1 cl1), TV (VPi vA2 cl2) =>
+      r (TV vA1) (TV vA2) /\ r (TC cl1) (TC cl2)
+
+  (* Eta/extensionality: relate Lam and Pi by observing evaluations of bodies.
+     We encode the observational clause operationally: for all args, whenever
+     both bodies evaluate in their respective extended envs to r1,r2, those results
+     must be related by r (as TV). *)
+(*   | TV (VLam vA1 cl1), TV (VPi vA2 cl2) =>
+      r (TV vA1) (TV vA2) /\
+      (forall (arg : whnf) (r1 r2 : whnf),
+         eval' (arg :: env_of_cl cl1) (body_of_cl cl1) r1 ->
+         eval' (arg :: env_of_cl cl2) (body_of_cl cl2) r2 ->
+         r (TV r1) (TV r2))
+
+  | TV (VPi vA1 cl1), TV (VLam vA2 cl2) =>
+      r (TV vA1) (TV vA2) /\
+      (forall (arg : whnf) (r1 r2 : whnf),
+         eval' (arg :: env_of_cl cl1) (body_of_cl cl1) r1 ->
+         eval' (arg :: env_of_cl cl2) (body_of_cl cl2) r2 ->
+         r (TV r1) (TV r2)) *)
+
+  (* closure case *)
+  | TC (Cl ρ1 t1), TC (Cl ρ2 t2) =>
+      Forall2 (fun x y => r (TV x) (TV y)) ρ1 ρ2 /\
+      (forall (arg : whnf) (r1 : whnf),
+         eval' (arg :: ρ1) t1 r1 ->
+         exists r2, eval' (arg :: ρ2) t2 r2 /\ r (TV r1) (TV r2)) /\
+      (forall (arg : whnf) (r2 : whnf),
+         eval' (arg :: ρ2) t2 r2 ->
+         exists r1, eval' (arg :: ρ1) t1 r1 /\ r (TV r1) (TV r2))
+
+  (* other combinations are false (different shapes cannot be related by one step) *)
+  | _, _ => False
+  end.
+
+Definition conv := paco2 convF bot2.
+
+Lemma conv_refl: forall v, conv v v.
+Proof. pcofix CIH.
+       intro v.
+       induction v; intros.
+       - pfold. simpl. destruct n.
+         + easy.
+         + split. right. apply CIH.
+           right. apply CIH.
+         + split. right. apply CIH.
+           split. right. apply CIH.
+           split. right. apply CIH.
+           right. apply CIH.
+         + split. right. apply CIH.
+           split. right. apply CIH.
+           split. right. apply CIH.
+           split. right. apply CIH.
+           right. apply CIH.
+       - pfold. simpl.
+         destruct w; try easy.
+         + split. right. apply CIH.
+           right. apply CIH.
+         + split. right. apply CIH.
+           right. apply CIH.
+         + right. apply CIH.
+         + right. apply CIH.
+         + split. right. apply CIH.
+           right. apply CIH.
+         + right. apply CIH.
+         + split. right. apply CIH.
+           split. right. apply CIH.
+           split. right. apply CIH.
+           right. apply CIH.
+       - pfold. simpl.
+         destruct c.
+         split.
+         induction l; intros.
+         + constructor.
+         + constructor. right. apply CIH.
+           apply IHl.
+         + intros. split.
+           intros. exists r1. split. easy.
+           right. apply CIH.
+           intros.
+           exists r2. split. easy.
+           right. apply CIH.
+Qed.
+
+Lemma Forall2_conv_sym: forall l s r,
+  (forall v1 v2 : conv_tag, conv v1 v2 -> r v2 v1) -> 
+  Forall2 (fun x y : whnf => upaco2 convF bot2 (TV x) (TV y)) l s ->
+  Forall2 (fun x y : whnf => upaco2 convF r (TV x) (TV y)) s l.
+Proof. intro l.
+       induction l; intros.
+       - inversion H0. constructor.
+       - inversion H0. subst.
+         constructor.
+         right. apply H.
+         destruct H3; easy.
+         apply IHl; easy.
+Qed.
+
+Lemma Forall2_conv_trans: forall l s u r,
+  (forall v1 v2 v3: conv_tag, conv v1 v2 -> conv v2 v3 -> r v1 v3) -> 
+  Forall2 (fun x y : whnf => upaco2 convF bot2 (TV x) (TV y)) l s ->
+  Forall2 (fun x y : whnf => upaco2 convF bot2 (TV x) (TV y)) s u ->
+  Forall2 (fun x y : whnf => upaco2 convF r (TV x) (TV y)) l u.
+Proof. intro l.
+       induction l; intros.
+       - inversion H0. subst. inversion H1. subst. constructor.
+       - inversion H0. subst. inversion H1. subst.
+         constructor.
+         right. apply H with (v2 := (TV y)).
+         destruct H4; easy.
+         destruct H5; easy.
+         apply IHl with (s := l'); easy.
+Qed.
+
+Lemma Forall2_LE: forall l s r r',
+  (forall x0 x1 : conv_tag, r x0 x1 -> r' x0 x1) ->
+  Forall2 (fun x y : whnf => r (TV x) (TV y)) l s ->
+  Forall2 (fun x y : whnf => r' (TV x) (TV y)) l s.
+Proof. intro l.
+       induction l; intros.
+       - inversion H0. constructor.
+       - inversion H0. subst.
+         constructor. apply H; easy.
+         apply IHl with (r := r); easy.
+Qed.
+
+Lemma mon_convF: monotone2 convF.
+Proof. unfold monotone2.
+       intro v1.
+       induction v1; intros.
+       - case_eq x1; intros.
+         + subst. simpl in IN.
+           destruct n, n0; try easy.
+           simpl.
+           split. apply LE; easy. apply LE; easy.
+           simpl.
+           split. apply LE; easy. split. apply LE; easy.
+           split. apply LE; easy. apply LE; easy.
+           simpl.
+           split. apply LE; easy. split. apply LE; easy.
+           split. apply LE; easy. split. apply LE; easy.
+           apply LE; easy.
+         + subst.
+           simpl in IN. destruct n; easy.
+         + subst.
+           simpl in IN. destruct n; easy.
+        - case_eq x1; intros.
+          + subst.
+            simpl in IN. destruct w; easy.
+          + subst.
+            simpl in IN. destruct w, w0; try easy.
+            * simpl.
+              split. apply LE; easy. apply LE; easy.
+            * simpl.
+              split. apply LE; easy. apply LE; easy.
+            * simpl. apply LE; easy.
+            * simpl. apply LE; easy.
+            * simpl. 
+              split. apply LE; easy. apply LE; easy.
+            * simpl. apply LE; easy.
+            * simpl. 
+              split. apply LE; easy. split. apply LE; easy.
+              split. apply LE; easy. apply LE; easy.
+          + subst.
+            simpl in IN. destruct w; easy.
+        - case_eq x1; intros.
+          + subst.
+            simpl in IN. destruct c; easy.
+          + subst.
+            simpl in IN. destruct c; easy.
+          + subst.
+            simpl in IN. simpl.
+            destruct c, c0.
+            destruct IN as (Ha,(Hb,Hc)).
+            split.
+            apply Forall2_LE with (r := r); easy.
+            split.
+            intros.
+            apply Hb in H.
+            destruct H as (res2,(Hr2,Hr3)).
+            exists res2. split. easy.
+            apply LE; easy.
+            intros.
+            apply Hc in H.
+            destruct H as (res2,(Hr2,Hr3)).
+            exists res2. split. easy.
+            apply LE; easy.
+Qed.
+
+Lemma conv_sym: forall v1 v2, conv v1 v2 -> conv v2 v1.
+Proof. pcofix CIH.
+       intro v1.
+       induction v1; intros.
+       3:{
+       case_eq v2; intros.
+       - subst. punfold H0. simpl in H0.
+         destruct c. easy.
+         apply mon_convF.
+       - subst. punfold H0. simpl in H0.
+         destruct c. easy.
+         apply mon_convF.
+       - subst. punfold H0. simpl in H0.
+         destruct c, c0.
+         destruct H0 as (Ha,(Hb,Hc)).
+         pfold. simpl. split.
+         apply Forall2_conv_sym; easy.
+         split.
+         intros.
+         apply Hc in H.
+         destruct H as (res,H).
+         exists res. split. easy.
+         right.
+         apply CIH. 
+         destruct H as (Hn,Hm).
+         destruct Hm as [Hm |Hm]. easy. easy.
+         intros.
+         apply Hb in H.
+         destruct H as (res,H).
+         exists res. split. easy.
+         right.
+         apply CIH. 
+         destruct H as (Hn,Hm).
+         destruct Hm as [Hm |Hm]. easy. easy.
+         apply mon_convF.
+       }
+       - case_eq v2; intros.
+         + subst. punfold H0. pfold.
+           simpl in *.
+           destruct n.
+           ++ destruct n0. easy.
+              easy.
+              easy.
+              easy.
+           ++ destruct n0; try easy.
+              destruct H0 as (Ha,Hb).
+              split.
+              * unfold upaco2 in Ha.
+                destruct Ha as [Ha | Ha].
+                ** right. apply CIH. easy.
+                ** easy.
+              * destruct Hb as [Hb | Hb].
+                ** right. apply CIH. easy.
+                ** easy.
+           ++ destruct n0; try easy.
+              destruct H0 as (Ha,(Hb,(Hc,Hd))).
+              split.
+              right. apply CIH.
+              destruct Ha; easy.
+              split.
+              right. apply CIH.
+              destruct Hb; easy.
+              split.
+              right. apply CIH.
+              destruct Hc; easy.
+              right. apply CIH.
+              destruct Hd; easy.
+           ++ destruct n0; try easy.
+              destruct H0 as (Ha,(Hb,(Hc,(Hd,He)))).
+              split.
+              right. apply CIH.
+              destruct Ha; easy.
+              split.
+              right. apply CIH.
+              destruct Hb; easy.
+              split.
+              right. apply CIH.
+              destruct Hc; easy.
+              split.
+              right. apply CIH.
+              destruct Hd; easy.
+              right. apply CIH.
+              destruct He; easy.
+            ++ apply mon_convF.
+         + subst.
+           punfold H0. simpl in H0. destruct n; easy.
+           apply mon_convF.
+         + subst.
+           punfold H0. simpl in H0. destruct n; easy.
+           apply mon_convF.
+       - case_eq v2; intros.
+         + subst.
+           punfold H0. simpl in H0. destruct w; easy.
+           apply mon_convF.
+         + subst. 
+           punfold H0. simpl in H0. pfold. simpl.
+           destruct w, w0; try easy.
+           ++ destruct H0 as (Ha,Hb).
+              split.
+              right. apply CIH.
+              destruct Ha; easy.
+              right. apply CIH.
+              destruct Hb; easy.
+           ++ destruct H0 as (Ha,Hb).
+              split.
+              right. apply CIH.
+              destruct Ha; easy.
+              right. apply CIH.
+              destruct Hb; easy.
+           ++ right. apply CIH.
+              destruct H0; easy.
+           ++ right. apply CIH.
+              destruct H0; easy.
+           ++ destruct H0 as (Ha,Hb).
+              split.
+              right. apply CIH.
+              destruct Ha; easy.
+              right. apply CIH.
+              destruct Hb; easy.
+           ++ right. apply CIH.
+              destruct H0; easy.
+           ++ destruct H0 as (Ha,(Hb,(Hc,Hd))).
+              split.
+              right. apply CIH.
+              destruct Ha; easy.
+              split.
+              right. apply CIH.
+              destruct Hb; easy.
+              split.
+              right. apply CIH.
+              destruct Hc; easy.
+              right. apply CIH.
+              destruct Hd; easy.
+           ++ apply mon_convF.
+         + subst.
+           punfold H0. simpl in H0. destruct w; easy.
+           apply mon_convF.
+Qed.
+
+Lemma conv_trans: forall v1 v2 v3, conv v1 v2 -> conv v2 v3 -> conv v1 v3.
+Proof. pcofix CIH.
+       intro v1.
+       induction v1; intros.
+       3:{
+       case_eq v2; intros.
+       - subst. punfold H0. simpl in H0.
+         destruct c. easy.
+         apply mon_convF.
+       - subst. punfold H0. simpl in H0.
+         destruct c. easy.
+         apply mon_convF.
+       - subst.
+         case_eq v3; intros.
+         + subst. punfold H1. simpl in H1.
+           destruct c0. easy.
+           apply mon_convF.
+         + subst. punfold H1. simpl in H1.
+           destruct c0. easy.
+           apply mon_convF.
+         + subst.
+           punfold H0. punfold H1.
+           simpl in H0, H1.
+           destruct c0, c, c1.
+           pfold. simpl.
+           destruct H1 as (H1a,(H1b,H1c)).
+           destruct H0 as (H2a,(H2b,H2c)).
+           split.
+           apply Forall2_conv_trans with (s := l); easy.
+           split.
+           intros.
+           apply H2b in H.
+           destruct H as (res2,(Hm,Hn)).
+           apply H1b in Hm.
+           destruct Hm as (res3,(Hm,Ho)).
+           exists res3. split. easy.
+           right. apply CIH with (v2 := (TV res2)).
+           destruct Hn; easy.
+           destruct Ho; easy.
+           intros.
+           apply H1c in H.
+           destruct H as (res2,(Hm,Hn)).
+           apply H2c in Hm.
+           destruct Hm as (res3,(Hm,Ho)).
+           exists res3. split. easy.
+           right. apply CIH with (v2 := (TV res2)).
+           destruct Ho; easy.
+           destruct Hn; easy.
+           apply mon_convF.
+           apply mon_convF.
+         }
+         - case_eq v2; intros.
+           + subst.
+             case_eq v3; intros.
+             ++ subst.
+                pfold. punfold H0. punfold H1. simpl in *.
+                destruct n, n0, n1; try easy.
+                * subst. easy.
+                * destruct H1 as (Ha,Hb).
+                  destruct H0 as (Hc,Hd).
+                  split.
+                  right. apply CIH with (v2 := (TNe n0)).
+                  destruct Hc; easy.
+                  destruct Ha; easy.
+                  right. apply CIH with (v2 := (TV w0)).
+                  destruct Hd; easy.
+                  destruct Hb; easy.
+                * destruct H1 as (Ha,(Hb,(Hc,Hd))).
+                  destruct H0 as (He,(Hf,(Hg,Hh))).
+                  split.
+                  right. apply CIH with (v2 := (TV w2)).
+                  destruct He; easy.
+                  destruct Ha; easy.
+                  split.
+                  right. apply CIH with (v2 := (TV w3)).
+                  destruct Hf; easy.
+                  destruct Hb; easy.
+                  split.
+                  right. apply CIH with (v2 := (TV w4)).
+                  destruct Hg; easy.
+                  destruct Hc; easy.
+                  right. apply CIH with (v2 := (TNe n0)).
+                  destruct Hh; easy.
+                  destruct Hd; easy.
+                * destruct H1 as (Ha,(Hb,(Hc,(Hd,He)))).
+                  destruct H0 as (Hf,(Hg,(Hh,(Hi,Hj)))).
+                  split.
+                  right. apply CIH with (v2 := (TV w3)).
+                  destruct Hf; easy.
+                  destruct Ha; easy.
+                  split.
+                  right. apply CIH with (v2 := (TV w4)).
+                  destruct Hg; easy.
+                  destruct Hb; easy.
+                  split.
+                  right. apply CIH with (v2 := (TV w5)).
+                  destruct Hh; easy.
+                  destruct Hc; easy.
+                  split.
+                  right. apply CIH with (v2 := (TV w6)).
+                  destruct Hi; easy.
+                  destruct Hd; easy.
+                  right. apply CIH with (v2 := (TNe n0)).
+                  destruct Hj; easy.
+                  destruct He; easy.
+                * apply mon_convF.
+                * apply mon_convF.
+             ++ subst.
+                punfold H1. simpl in H1. destruct n0; easy.
+                apply mon_convF.
+             ++ subst.
+                punfold H1. simpl in H1. destruct n0; easy.
+                apply mon_convF.
+           + subst. 
+             punfold H0. simpl in H0. destruct n; easy.
+             apply mon_convF.
+           + subst. 
+             punfold H0. simpl in H0. destruct n; easy.
+             apply mon_convF.
+         - case_eq v2; intros.
+           + subst. 
+             punfold H0. simpl in H0. destruct w; easy.
+             apply mon_convF.
+           + subst.
+             case_eq v3; intros.
+             ++ subst.
+                punfold H1. simpl in H1. destruct w0; easy.
+                apply mon_convF.
+             ++ subst.
+                pfold. punfold H0. punfold H1. simpl in *.
+                destruct w, w0, w1; try easy.
+                * destruct H1 as (Ha,Hb).
+                  destruct H0 as (Hc,Hd).
+                  split.
+                  right. apply CIH with (v2 := (TV w0)).
+                  destruct Hc; easy.
+                  destruct Ha; easy.
+                  right. apply CIH with (v2 := (TC c0)).
+                  destruct Hd; easy.
+                  destruct Hb; easy.
+                * destruct H1 as (Ha,Hb).
+                  destruct H0 as (Hc,Hd).
+                  split.
+                  right. apply CIH with (v2 := (TV w0)).
+                  destruct Hc; easy.
+                  destruct Ha; easy.
+                  right. apply CIH with (v2 := (TC c0)).
+                  destruct Hd; easy.
+                  destruct Hb; easy.
+                * right. apply CIH with (v2 := (TV w0)).
+                  destruct H0; easy.
+                  destruct H1; easy.
+                * right. apply CIH with (v2 := (TNe n0)).
+                  destruct H0; easy.
+                  destruct H1; easy.
+                * destruct H1 as (Ha,Hb).
+                  destruct H0 as (Hc,Hd).
+                  split.
+                  right. apply CIH with (v2 := (TV w0_1)).
+                  destruct Hc; easy.
+                  destruct Ha; easy.
+                  right. apply CIH with (v2 := (TV w0_2)).
+                  destruct Hd; easy.
+                  destruct Hb; easy.
+                * right. apply CIH with (v2 := (TV w0)).
+                  destruct H0; easy.
+                  destruct H1; easy.
+                * destruct H1 as (Ha,(Hb,(Hc,Hd))).
+                  destruct H0 as (He,(Hf,(Hg,Hh))).
+                  split.
+                  right. apply CIH with (v2 := (TV w0_1)).
+                  destruct He; easy.
+                  destruct Ha; easy.
+                  split.
+                  right. apply CIH with (v2 := (TV w0_2)).
+                  destruct Hf; easy.
+                  destruct Hb; easy.
+                  split.
+                  right. apply CIH with (v2 := (TV w0_3)).
+                  destruct Hg; easy.
+                  destruct Hc; easy.
+                  right. apply CIH with (v2 := (TV w0_4)).
+                  destruct Hh; easy.
+                  destruct Hd; easy.
+                * apply mon_convF.
+                * apply mon_convF.
+             ++ subst.
+                punfold H1. simpl in H1. destruct w0; easy.
+                apply mon_convF.
+           + subst.
+             punfold H0. simpl in H0. destruct w; easy.
+             apply mon_convF.
+Qed.
+
+Definition neutral_conv (n1 n2 : neutral) : Prop := conv (TNe n1) (TNe n2).
+Definition vconv (v1 v2 : whnf) : Prop := conv (TV v1) (TV v2).
+Definition closure_conv (c1 c2 : closure) : Prop := conv (TC c1) (TC c2).
+
+(* Assumes the code you gave above (term, whnf, neutral, closure, eval', eval_natrec, eval_vecrec, vconv, closure_conv) is already present. *)
+
+Section BidirectionalTyping.
+
+  (* Context: list of whnf (value-types) *)
+  Definition ctx := list whnf.
+
+  (* Helper: lookup in ctx *)
+  Definition ctx_lookup (Γ : ctx) (n : nat) : option whnf := nth_error Γ n.
+
+
+Reserved Notation "Γ ⊢ₛ t ⇑ A" (at level 70).
+Reserved Notation "Γ ⊢𝚌 t ⇓ A" (at level 70).
+
+(* syntactic shape predicate for type-level terms (useful in progress hypotheses) *)
+Inductive is_type_shape : term -> Prop :=
+| ITS_Star : is_type_shape Star
+| ITS_Nat  : is_type_shape Nat
+| ITS_Var  : forall x, is_type_shape (Var x)
+| ITS_App : forall t u, is_type_shape t -> is_type_shape (App t u)
+| ITS_Pi   : forall A B, is_type_shape A -> is_type_shape B -> is_type_shape (Pi A B)
+| ITS_Vec  : forall A n, is_type_shape A -> is_type_shape (Vec A n)
+| ITS_NatRec : forall P z s n, is_type_shape P -> is_type_shape (NatRec P z s n)
+| ITS_VecRec : forall P nil cons n t, is_type_shape P -> is_type_shape (VecRec P nil cons n t).
+
+(* ---------------------------
+   Bidirectional typing
+   --------------------------- *)
+
+Inductive synth : ctx -> term -> whnf -> Prop :=
+  (* variables: types are stored as whnf in the context *)
+| S_Var : forall Γ x A,
+    nth_error Γ x = Some A ->
+    synth Γ (Var x) A
+
+  (* universes / base types *)
+| S_Star : forall Γ,
+    synth Γ Star VStar
+
+| S_Nat : forall Γ,
+    synth Γ Nat VNat
+
+  (* Pi formation: domain must evaluate to a type, and codomain must check as a type
+     under the extended static context (vdom :: Γ).  The produced WHNF is the Pi
+     whose closure captures the *syntactic* codomain term in context Γ. *)
+| S_Pi : forall Γ A B vA,
+    eval' Γ A vA ->                (* evaluate domain annotation *)
+    vconv vA VStar ->               (* domain is a type *)
+    check (vA :: Γ) B VStar ->      (* codomain is a type under the extended static context *)
+    synth Γ (Pi A B) (VPi vA (Cl Γ B))
+
+  (* Application: synthesize t to something convertible to VPi vdom clB,
+     evaluate u to vu, and evaluate the body under the closure to get result type *)
+| S_App : forall Γ t u vt vu vdom clB ρB Bterm vres,
+    synth Γ t vt ->
+    eval' Γ u vu ->
+    vconv vt (VPi vdom clB) ->
+    clB = Cl ρB Bterm ->
+    eval' (vu :: ρB) Bterm vres ->
+    synth Γ (App t u) vres
+
+  (* Zero & Succ *)
+| S_Zero : forall Γ, synth Γ Zero VNat
+
+| S_Succ : forall Γ n,
+    check Γ n VNat ->
+    synth Γ (Succ n) VNat
+
+  (* NatRec (term-level eliminator): result is whatever eval_natrec returns *)
+| S_NatRec_term : forall Γ P z s n vP vz vs vn v,
+    eval' Γ P vP ->
+    eval' Γ z vz ->
+    eval' Γ s vs ->
+    eval' Γ n vn ->
+    eval_natrec vP vz vs vn v ->
+    synth Γ (NatRec P z s n) v
+
+  (* Vec formation: components must be types (A : VStar) and index a Nat *)
+| S_Vec : forall Γ A n vA vn,
+    eval' Γ A vA ->
+    vconv vA VStar ->
+    eval' Γ n vn ->
+    vconv vn VNat ->
+    synth Γ (Vec A n) (VVec vA vn)
+
+  (* Nil / Cons synthesize the *type* of the vector, not the value *)
+| S_Nil : forall Γ A vA,
+    eval' Γ A vA ->
+    vconv vA VStar ->
+    synth Γ (Nil A) (VVec vA VZero)
+
+| S_Cons : forall Γ A n x xs vA vn,
+    eval' Γ A vA ->
+    vconv vA VStar ->
+    eval' Γ n vn ->
+    vconv vn VNat ->
+    check Γ x vA ->                       (* x : A *)
+    check Γ xs (VVec vA vn) ->            (* xs : Vec A n *)
+    synth Γ (Cons A n x xs) (VVec vA (VSucc vn))
+
+  (* VecRec term-level synthesizer *)
+| S_VecRec_term : forall Γ P nil cons n t vt vP vnil vcons vn vres,
+    eval' Γ P vP ->
+    eval' Γ nil vnil ->
+    eval' Γ cons vcons ->
+    eval' Γ n vn ->
+    eval' Γ t vt ->
+    eval_vecrec vP vnil vcons vn vt vres ->
+    synth Γ (VecRec P nil cons n t) vres
+
+  (* Annotated lambda (synthesizes a Pi based on annotation). We require the annotation
+     to synthesize to a type (vdom) and that the lambda body checks under the extended
+     static context (vdom :: Γ) to some vB; the produced Pi closure captures the
+     body-as-term with Γ. *)
+| S_Lam_Ann : forall Γ annA b vdom vB,
+    synth Γ annA vdom ->
+    vconv vdom VStar ->
+    check (vdom :: Γ) b vB ->
+    synth Γ (Lam annA b) (VPi vdom (Cl Γ b))
+
+where "Γ ⊢ₛ t ⇑ A" := (synth Γ t A)
+
+with check : ctx -> term -> whnf -> Prop :=
+(* checking by synth + convert *)
+| C_Synth : forall Γ t A' A,
+    synth Γ t A' ->
+    vconv A' A ->
+    check Γ t A
+
+(* check lambda against expected Pi: expected A convertible to Pi vdom clB,
+   evaluate the expected codomain under clB's env to get vB, check the lambda body
+   under its own static environment (vdom :: Γ) against that vB, then require
+   the runtime closure produced by the lambda be observationally convertible to clB. *)
+| C_Lam : forall Γ (A : whnf) annA b vdom clB ρB Bterm vB,
+    synth Γ annA vdom ->                 (* annotation synthesizes the domain *)
+    vconv vdom VStar ->                  (* annotation must be a type *)
+    vconv A (VPi vdom clB) ->            (* expected type convertible to Pi vdom clB *)
+    clB = Cl ρB Bterm ->
+    eval' (vdom :: ρB) Bterm vB ->       (* evaluate codomain under clB's runtime env *)
+    check (vdom :: Γ) b vB ->            (* check the lambda body in its own static env *)
+    closure_conv (Cl Γ b) clB ->         (* closures must be observationally convertible *)
+    check Γ (Lam annA b) A
+
+(* NatRec checked against an expected A: evaluate elim components and require the
+   evaluation of the elimination be convertible to A *)
+| C_NatRec_check : forall Γ P z s n A vP vz vs vn v,
+    eval' Γ P vP ->
+    eval' Γ z vz ->
+    eval' Γ s vs ->
+    eval' Γ n vn ->
+    eval_natrec vP vz vs vn v ->
+    vconv v A ->
+    check Γ (NatRec P z s n) A
+
+(* VecRec checked against expected A *)
+| C_VecRec_check : forall Γ P nil cons n A t vt vP vnil vcons vn vres,
+    eval' Γ P vP ->
+    eval' Γ nil vnil ->
+    eval' Γ cons vcons ->
+    eval' Γ n vn ->
+    eval' Γ t vt ->
+    eval_vecrec vP vnil vcons vn vt vres ->
+    vconv vres A ->
+    check Γ (VecRec P nil cons n t) A
+
+where "Γ ⊢𝚌 t ⇓ A" := (check Γ t A).
+
+Scheme synth_rect := Induction for synth Sort Prop
+with check_rect := Induction for check Sort Prop.
+
+Combined Scheme typing_mutind from synth_rect, check_rect.
+
+(* Lemma typing_unique_mut :
+  (forall Γ t A (He : synth Γ t A) A' (He' : synth Γ t A'), vconv A A')  /\
+  (forall Γ t A (He : check Γ t A) A' (He' : synth Γ t A'), vconv A A').
+Proof.
+  eapply (typing_mutind
+    (fun Γ t A (He : synth Γ t A) => forall A' (He' : synth Γ t A'), vconv A A')
+    (fun Γ t A (He : check Γ t A) => forall A' (He' : synth Γ t A'), vconv A A')
+  ).
+  17:{
+  intros.
+  inversion He'. subst.
+  assert(vres = A') by admit.
+  subst.
+  admit.
+  }
+Admitted. *)
+
+Lemma synth_preserve_eval_for_types :
+  (forall Γ t A (He : synth Γ t A),
+    forall v, is_type_shape t -> eval' Γ t v -> vconv A v)
+  /\
+  (forall Γ t A (He : check Γ t A),
+     forall v, is_type_shape t -> eval' Γ t v -> vconv A v).
+Proof.
+  eapply (typing_mutind
+    (fun (Γ : ctx) (t : term) (A : whnf) (He : synth Γ t A) =>
+       forall v, is_type_shape t -> eval' Γ t v -> vconv A v)
+    (fun (Γ : ctx) (t : term) (A : whnf) (He : check Γ t A) =>
+       forall v, is_type_shape t -> eval' Γ t v -> vconv A v)
+  ).
+  17:{
+  intros.
+  inversion H0. subst.
+  assert(v0 = vres).
+  { specialize(eval'_det  _ _ _ _ e H6); intro HHa.
+    specialize(eval'_det  _ _ _ _ e0 H8); intro HHb.
+    specialize(eval'_det  _ _ _ _ e1 H10); intro HHc.
+    specialize(eval'_det  _ _ _ _ e2 H11); intro HHd.
+    specialize(eval'_det  _ _ _ _ e3 H12); intro HHe.
+    subst.
+    specialize(eval_vecrec_det _ _ _ _ _ _ _ e4 H13); intro HHf.
+    easy.
+  }
+  subst.
+  apply conv_sym. easy.
+  }
+  16:{
+  intros.
+  inversion H0. subst.
+  assert(v = v1).
+  { specialize(eval'_det  _ _ _ _ e H5); intro HHa.
+    specialize(eval'_det  _ _ _ _ e0 H7); intro HHb.
+    specialize(eval'_det  _ _ _ _ e1 H9); intro HHc.
+    specialize(eval'_det  _ _ _ _ e2 H10); intro HHd.
+    subst.
+    specialize(eval_natrec_det _ _ _ _ _ _ e3 H11); intro HHf.
+    easy.
+  }
+  subst.
+  apply conv_sym. easy.
+  }
+  15:{
+  intros.
+  inversion H2. subst.
+  inversion H1.
+  }
+  14:{
+  intros.
+  apply H with (v := v0) in H0.
+  apply conv_sym in v.
+  apply conv_trans with (v2 := (TV A')); easy.
+  easy.
+  }
+  13:{
+  intros.
+  inversion H1.
+  }
+  12:{
+  intros.
+  inversion H0. subst.
+  assert(v = vres).
+  { specialize(eval'_det  _ _ _ _ e H6); intro HHa.
+    specialize(eval'_det  _ _ _ _ e0 H8); intro HHb.
+    specialize(eval'_det  _ _ _ _ e1 H10); intro HHc.
+    specialize(eval'_det  _ _ _ _ e2 H11); intro HHd.
+    specialize(eval'_det  _ _ _ _ e3 H12); intro HHe.
+    subst.
+    specialize(eval_vecrec_det _ _ _ _ _ _ _ e4 H13); intro HHf.
+    easy.
+  }
+  subst.
+  apply conv_refl.
+  }
+  11:{
+  intros. inversion H1.
+  }
+  10:{
+  intros. inversion H.
+  }
+  9:{
+  intros. inversion H0. subst.
+  assert(vA = vA0).
+  { specialize(eval'_det  _ _ _ _ e H4); intro HHa.
+    specialize(eval'_det  _ _ _ _ e0 H6); intro HHb.
+    subst.
+    easy.
+  }
+  assert(vn = vn0).
+  { specialize(eval'_det  _ _ _ _ e0 H6); intro HHb.
+    subst. easy.
+  }
+  subst. 
+  apply conv_refl.
+  }
+  8:{
+  intros.
+  inversion H0. subst.
+  assert(v0 = v).
+  { specialize(eval'_det  _ _ _ _ e H5); intro HHa.
+    specialize(eval'_det  _ _ _ _ e0 H7); intro HHb.
+    specialize(eval'_det  _ _ _ _ e1 H9); intro HHc.
+    specialize(eval'_det  _ _ _ _ e2 H10); intro HHd.
+    subst.
+    specialize(eval_natrec_det _ _ _ _ _ _ e3 H11); intro HHf.
+    easy.
+  }
+  subst.
+  apply conv_refl.
+  }
+  7:{
+  intros. inversion H0.
+  }
+  6:{
+  intros. inversion H.
+  }
+  5:{
+  intros.
+  inversion H0. subst.
+  inversion H1. subst.
+  specialize(H vt0 H3 H5).
+  assert(vconv vt0 (VPi vdom (Cl ρB Bterm))).
+  { apply conv_sym in H.
+    apply conv_trans with (v2 := (TV vt)); easy.
+  }
+  punfold H2. simpl in H2.
+  destruct vt0; try easy.
+  destruct H2 as (Ha,Hb).
+  destruct Ha as [Ha | Ha].
+  punfold H.
+  simpl in H.
+  destruct vt; try easy.
+  destruct H as (Hc,Hd).
+  inversion H9.
+  subst.
+  destruct Hb as [Hb | Hb].
+  punfold Hb. simpl in Hb.
+  destruct Hb as (Hb1,Hb2).
+  assert(vu = vu0).
+  { specialize(eval'_det  _ _ _ _ e H7); intro HHa.
+    easy.
+  }
+  subst.
+  destruct Hb2 as (Hb21,Hb22).
+  apply Hb22 in e1.
+  destruct e1 as (res1,(He1,He2)).
+  apply Hb21 in H8.
+  destruct H8 as (res2,(He3,He4)).
+  inversion H9. subst.
+  assert(v0 = res1).
+  { specialize(eval'_det  _ _ _ _ He1 H10); intro HHa.
+    easy.
+  }
+  subst.
+  destruct He2 as [He2 | He2].
+  apply conv_sym in He2.
+  easy.
+  easy.
+  apply mon_convF.
+  easy.
+  apply mon_convF.
+  easy.
+  apply mon_convF.
+ }
+ 4:{
+ intros.
+ inversion H0. subst.
+ inversion H1. subst.
+ assert(vA = vA0).
+ { specialize(eval'_det  _ _ _ _ e H8); intro HHa.
+   easy.
+  }
+ subst.
+ pfold. simpl.
+ split. left. apply conv_refl.
+ left. apply conv_refl.
+ }
+ 3:{
+ intros.
+ inversion H0. subst.
+ apply conv_refl.
+ }
+ 2:{
+ intros.
+ inversion H0. apply conv_refl.
+ }
+ 1:{
+ intros.
+ inversion H0.
+ + subst. rewrite e in H3. inversion H3. apply conv_refl.
+ + subst. rewrite e in H3. easy.
+ }
+Qed.
+
+Lemma synth_preserve_eval :
+  forall Γ t A v,
+    is_type_shape t ->
+    eval' Γ t v ->
+    synth Γ t A ->
+    vconv A v.
+Proof.
+  intros Γ t A v Hclosed Heval Hs.
+  eapply (proj1 synth_preserve_eval_for_types); eauto.
+Qed.
+
+Lemma check_preserve_eval :
+  forall Γ t A v,
+    is_type_shape t ->
+    eval' Γ t v ->
+    check Γ t A ->
+    vconv A v.
+Proof.
+  intros Γ t A v Hclosed Heval Hc.
+  eapply (proj2 synth_preserve_eval_for_types); eauto.
+Qed.
+
+Lemma progress_mut :
+  (forall Γ t A (Hs : synth Γ t A),  Γ = [] -> is_type_shape t -> exists v, eval' [] t v)
+  /\
+  (forall Γ t A (Hc : check Γ t A),  Γ = [] -> is_type_shape t ->  exists v, eval' [] t v).
+Proof.
+  (* use predicates that mention Γ so typing_mutind can accept them,
+     but require Γ = [] inside the predicate *)
+  eapply (typing_mutind
+    (fun (Γ : ctx) (t : term) (A : whnf) (He : synth Γ t A) =>
+       Γ = [] -> is_type_shape t -> exists v, eval' [] t v)
+    (fun (Γ : ctx) (t : term) (A : whnf) (He : check Γ t A) =>
+       Γ = [] -> is_type_shape t -> exists v, eval' [] t v)
+  ).
+  4:{
+  intros.
+  subst.
+  exists (VPi vA (Cl [] B)).
+  apply E'_Pi.
+  exact e.
+  }
+  4:{
+  intros. subst.
+  specialize(H eq_refl).
+  inversion H1. subst. apply H in H2.
+  destruct H2 as (vta, Hvta).
+  punfold v.
+  simpl in v.
+  destruct vt; try easy.
+  destruct v as (Ha,Hb).
+  destruct Ha as [Ha | Ha].
+  assert(vconv vta (VPi vt c)).
+  { inversion H1. subst.
+    specialize(synth_preserve_eval _ _ _ _ H2 Hvta s); intro HH.
+    apply conv_sym. easy.
+  }
+  punfold H0. simpl in H0.
+  destruct vta; try easy.
+  destruct H0 as (Hc,Hd).
+  destruct Hc as [Hc | Hc].
+
+  inversion Hvta.
+  + subst.
+    rewrite nth_error_nil in H0. easy.
+  + subst.
+    assert(ρB = []).
+    { destruct Hb as [Hb | Hb].
+      punfold Hb. simpl in Hb.
+      destruct c.
+      destruct Hb. 
+      destruct Hd as [Hd | Hd].
+      punfold Hd. simpl in Hd.
+      destruct Hd.
+      inversion H3. subst.
+      inversion H0. easy.
+      apply mon_convF.
+      easy.
+      apply mon_convF.
+      easy.
+    }
+    subst.
+    assert(HCC: paco2 convF bot2 (TC (Cl [] B)) (TC (Cl [] Bterm))).
+    { destruct Hd as [Hd | Hd].
+      destruct Hb as [Hb | Hb].
+      apply conv_trans with (v2 := (TC c)); easy.
+      easy. easy.
+    }
+    punfold HCC. simpl in HCC.
+    destruct HCC as (Hc1,(Hc2,Hc3)).
+    apply Hc3 in e1.
+    destruct e1 as (res1,(He1,He2)).
+    exists res1.
+    apply E'_App with (vt := (VPi vta (Cl [] B))) (vu := vu); try easy.
+    apply VApp_Pi_sharp with (body := B).
+    easy.
+    apply mon_convF.
+  + subst.
+    destruct c0.
+    assert(HCC: paco2 convF bot2 (TC (Cl l t)) (TC (Cl ρB Bterm))).
+    { destruct Hd as [Hd | Hd].
+      destruct Hb as [Hb | Hb].
+      apply conv_trans with (v2 := (TC c)); easy.
+      easy. easy.
+    }
+    punfold HCC. simpl in HCC.
+    destruct HCC as (Hc1,(Hc2,Hc3)).
+    apply Hc3 in e1.
+    destruct e1 as (res1,(He1,He2)).
+    exists res1.
+    apply E'_App with (vt := (VPi vta (Cl l t))) (vu := vu); try easy.
+    eapply VApp_Pi_sharp. easy.
+    apply mon_convF.
+   + subst.
+     destruct c0.
+     assert(HCC: paco2 convF bot2 (TC (Cl l t)) (TC (Cl ρB Bterm))).
+    { destruct Hd as [Hd | Hd].
+      destruct Hb as [Hb | Hb].
+      apply conv_trans with (v2 := (TC c)); easy.
+      easy. easy.
+    }
+     punfold HCC. simpl in HCC.
+     destruct HCC as (Hc1,(Hc2,Hc3)).
+     apply Hc3 in e1.
+     destruct e1 as (res1,(He1,He2)).
+     exists res1.
+     apply E'_App with (vt := (VPi vta (Cl l t))) (vu := vu); try easy.
+     eapply VApp_Pi_sharp. easy.
+     apply mon_convF.
+   + subst.
+     destruct c0.
+     assert(HCC: paco2 convF bot2 (TC (Cl l t)) (TC (Cl ρB Bterm))).
+    { destruct Hd as [Hd | Hd].
+      destruct Hb as [Hb | Hb].
+      apply conv_trans with (v2 := (TC c)); easy.
+      easy. easy.
+    }
+     punfold HCC. simpl in HCC.
+     destruct HCC as (Hc1,(Hc2,Hc3)).
+     apply Hc3 in e1.
+     destruct e1 as (res1,(He1,He2)).
+     exists res1.
+     apply E'_App with (vt := (VPi vta (Cl l t))) (vu := vu); try easy.
+     eapply VApp_Pi_sharp. easy.
+     apply mon_convF.
+   + easy.
+   + apply mon_convF.
+   + easy.
+   + apply mon_convF.
+  }
+  15:{
+  intros.
+  subst.
+  exists vres.
+  apply E'_VecRec with (vt:=vt) (vP:=vP) (vnil:=vnil) (vcons:=vcons) (vn:=vn).
+  all: auto.
+  }
+  14:{
+  intros.
+  subst.
+  exists v.
+  eapply E'_NatRec; eauto.
+  }
+  13:{
+  intros.
+  inversion H2.
+  }
+  12:{
+  intros.
+  subst. specialize(H eq_refl).
+  apply H in H1.
+  destruct H1 as (v1,H1).
+  exists v1. easy.
+  }
+  11:{
+  intros.
+  inversion H2.
+  }
+  10:{
+  intros. subst.
+  exists vres.
+  apply E'_VecRec with (vt:=vt) (vP:=vP) (vnil:=vnil) (vcons:=vcons) (vn:=vn); easy.
+  }
+  9:{
+  intros.
+  inversion H2.
+  }
+  8:{
+  intros.
+  inversion H0.
+  }
+  7:{
+  intros. subst.
+  exists (VVec vA vn).
+  apply E'_Vec; easy.
+  }
+  6:{
+  intros.
+  subst.
+  exists v.
+  eapply E'_NatRec; eauto.
+  }
+  5:{
+  intros.
+  inversion H1.
+  }
+  4:{
+  intros.
+  inversion H0.
+  }
+  3:{
+  intros.
+  subst.
+  exists VNat. 
+  apply E'_Nat.
+  }
+  2:{
+  intros.
+  subst.
+  exists VStar.
+  apply E'_Star.
+  }
+  1:{
+  intros.
+  subst.
+  rewrite nth_error_nil in e.
+  easy.
+  }
+Qed.
+
+Lemma synth_progress :
+  forall t A,
+    synth [] t A ->
+    is_type_shape t ->
+    exists v, eval' [] t v.
+Proof. 
+  intros t A Heq Hclosed.
+  eapply (proj1 progress_mut); eauto.
+Qed.
+
+Lemma check_progress :
+  forall t A,
+    check [] t A ->
+    is_type_shape t ->
+    exists v, eval' [] t v.
+Proof.
+  intros t A Heq Hclosed.
+  eapply (proj2 progress_mut); eauto.
+Qed.
+
+Theorem type_safety_mut :
+  (forall t A, synth [] t A -> is_type_shape t -> exists v, eval' [] t v /\ vconv A v)
+  /\
+  (forall t A, check [] t A -> is_type_shape t -> exists v, eval' [] t v /\ vconv A v).
+Proof.
+  split.
+  - intros t A Hs Hclosed.
+    (* progress for synth gives a value *)
+    destruct (synth_progress t A Hs Hclosed) as [v Hev].
+    (* preservation (synth_preserve_eval) gives convertibility of A and v *)
+    specialize (synth_preserve_eval [] t A v Hclosed Hev Hs).
+    exists v; split; auto.
+  - intros t A Hc Hclosed.
+    destruct (check_progress t A Hc Hclosed) as [v Hev].
+    specialize (check_preserve_eval [] t A v Hclosed Hev Hc).
+    exists v; split; auto.
+Qed.
+
+Lemma synth_type_safety :
+  forall t A,
+    synth [] t A ->
+    is_type_shape t ->
+    exists v, eval' [] t v /\ vconv A v.
+Proof.
+  intros t A Heq Hclosed.
+  eapply (proj1 type_safety_mut); eauto.
+Qed.
+
+Lemma check_type_safety :
+  forall t A,
+    check [] t A ->
+    is_type_shape t ->
+    exists v, eval' [] t v /\ vconv A v.
+Proof.
+  intros t A Heq Hclosed.
+  eapply (proj2 type_safety_mut); eauto.
+Qed.
+
+Definition add_term : term :=
+  Lam Nat
+    ( Lam Nat
+        ( NatRec
+            (Lam Nat Nat)                     (* P = λ_. Nat *)
+            (Var 0)                           (* z = y *)
+            (Lam Nat (Lam Nat (Succ (Var 0))))(* s = λn. λrec. Succ rec *)
+            (Var 1)                           (* n = x *)
+        )
+    ).
+
